src: Remove `Lem` from lemma names, reindent docstrings

src/Passes/SimplifyEmptyBlocks.dfy
@@ -90,7 +90,7 @@ module Bootstrap.Passes.SimplifyEmptyBlocks {
   import opened Transforms.Generic
   import opened Transforms.Proofs.BottomUp_
 
-  type {:verify false} Expr = Syntax.Expr
+  type Expr = Syntax.Expr
 
 module FilterCommon {
   import Utils.Lib
@@ -99,178 +99,27 @@ module FilterCommon {
   import opened AST.Syntax
   import opened Semantics.Equiv
   import opened Semantics.Interp
-  import opened Transforms.BottomUp // For the def of ``TODO()``
 
-  type {:verify false} Expr = Syntax.Expr
+  type Expr = Syntax.Expr
 
   // TODO: move?
-  predicate method {:verify false} IsEmptyBlock(e: Expr)
+  predicate method IsEmptyBlock(e: Expr)
   {
     e.Block? && e.stmts == []
   }
 
   // TODO: move?
-  predicate method {:verify false} IsNonEmptyBlock(e: Expr)
+  predicate method IsNonEmptyBlock(e: Expr)
   {
     !(IsEmptyBlock(e))
   }
 
-  // TODO: move
-  predicate Seq_All<T>(f: T -> bool, s: seq<T>)
-  {
-    forall x | x in s :: f(x)
-  }
-
-  predicate {:verify false} Tr_Expr_Post(e: Expr) {
+  predicate Tr_Expr_Post(e: Expr) {
     true
   }
 
-  predicate {:verify false} Tr_Expr_Rel(e: Expr, e': Expr) {
+  predicate Tr_Expr_Rel(e: Expr, e': Expr) {
     EqInterp(e, e')
-  }
-
-
-  // TODO: move
-  predicate {:verify false} EqInterpBlockExprs(es: seq<Exprs.T>, es': seq<Exprs.T>)
-  {
-    Seq_All(SupportsInterp, es) ==>
-    (&& Seq_All(SupportsInterp, es')
-     && forall env, ctx, ctx' | EqState(ctx, ctx') ::
-       EqInterpResultValue(
-                      InterpBlock_Exprs(es, env, ctx),
-                      InterpBlock_Exprs(es', env, ctx')))
-  }
-
-  // TODO: move
-  lemma {:verify false} EqInterpBlockExprs_Inst(es: seq<Exprs.T>, es': seq<Exprs.T>, env: Environment, ctx: State, ctx': State)
-    requires EqInterpBlockExprs(es, es')
-    requires Seq_All(SupportsInterp, es)
-    requires EqState(ctx, ctx')
-    ensures  EqInterpResultValue(InterpBlock_Exprs(es, env, ctx), InterpBlock_Exprs(es', env, ctx'))
-  {}
-  
-  // TODO: move
-  lemma {:verify false} InterpBlock_Exprs_Eq_Append(e: Expr, e': Expr, tl: seq<Expr>, tl': seq<Expr>, env: Environment, ctx: State, ctx': State)
-    requires SupportsInterp(e)
-    requires SupportsInterp(e')
-    requires Seq_All(SupportsInterp, tl)
-    requires Seq_All(SupportsInterp, tl')
-    requires EqState(ctx, ctx')
-    requires EqInterp(e, e')
-    requires EqInterpBlockExprs(tl, tl')
-    requires |tl| > 0
-    ensures EqInterpResultValue(InterpBlock_Exprs([e] + tl, env, ctx), InterpBlock_Exprs([e'] + tl', env, ctx'))
-    // Auxiliary lemma for the proofs about transformations operating on blocks. This is especially
-    // useful when those transformations might update the length of the sequence of expressions
-    // in the blocks. The proof is a bit tricky, because the case where the sequence has length 1
-    // is a special case in the definition of ``EqInterpBlock_Exprs``.
-  {
-    var es := [e] + tl;
-    var es' := [e'] + tl';
-    assert e == es[0];
-
-    reveal InterpBlock_Exprs();
-
-    // Evaluate the first expression
-    var res0 := InterpExpr(e, env, ctx);
-    var res0' := InterpExpr(e', env, ctx');
-    EqInterp_Lem(e, e', env, ctx, ctx');
-
-    // We need to make a case disjunction on whether the length of the concatenated sequences is
-    // > 1 or not
-    if |tl'| >= 1 {
-      // The "regular" case
-
-      // Evaluate the remaining expressions
-      if res0.Success? && res0.value.ret == V.Unit {
-        var Return(_, ctx0) := res0.value;
-        var Return(_, ctx0') := res0'.value;
-
-        var res1 := InterpBlock_Exprs(tl, env, ctx0);
-        var res1' := InterpBlock_Exprs(tl', env, ctx0');
-
-        EqInterpBlockExprs_Inst(tl, tl', env, ctx0, ctx0');
-      }
-      else {
-        // Trivial
-      }
-    }
-    else {
-      // Degenerate case
-      assert |tl'| == 0;
-
-      if res0.Success? {
-        var Return(v, ctx0) := res0.value;
-        var Return(v', ctx0') := res0'.value;
-
-        if v == V.Unit {
-          assert v' == V.Unit;
-          EqInterpBlockExprs_Inst(tl, tl', env, ctx0, ctx0');
-        }
-        else {
-          assert v' != V.Unit;
-
-          // TODO(SMH): update EqInterp so that this works (evaluating `es` will fail if `e` doesn't
-          // evaluate to `Unit`)
-          assume TODO();
-        }
-      }
-      else {
-        // Trivial
-      }
-    }
-  }
-
-  // TODO: move
-  predicate EqInterpResultValue_Strong(res: InterpResult<WV>, res': InterpResult<WV>) {
-    match (res, res') {
-      case (Success(Return(v,ctx)), Success(Return(v',ctx'))) =>
-        && v == v'
-        && ctx == ctx'
-      case (Failure(err), Failure(err')) =>
-        err == err'
-      case _ =>
-        false
-    }
-  }
-
-  // TODO: move
-  // TODO: remove? This lemma is trivial.
-  lemma {:verify false} InterpBlock_Exprs1_Strong_Eq(e: Expr, env: Environment, ctx: State)
-    requires SupportsInterp(e)
-    ensures EqInterpResultValue_Strong(InterpExpr(e, env, ctx), InterpBlock_Exprs([e], env, ctx))
-    // Auxiliary lemma: evaluating a block of one expression is equivalent to evaluating
-    // the single expression.
-  {
-    reveal InterpBlock_Exprs();
-  }
-
-  // TODO: move
-  lemma {:verify false} InterpBlock_Exprs_Refl(es: seq<Expr>, env: Environment, ctx: State, ctx': State)
-    requires Seq_All(SupportsInterp, es)
-    requires EqState(ctx, ctx')
-    ensures EqInterpResultValue(InterpBlock_Exprs(es, env, ctx), InterpBlock_Exprs(es, env, ctx'))
-  {
-    reveal InterpBlock_Exprs();
-    if es == [] {}
-    else {
-       // Evaluate the first expression
-      var res0 := InterpExpr(es[0], env, ctx);
-      var res0' := InterpExpr(es[0], env, ctx');
-      EqInterp_Refl_Lem(es[0]);
-      EqInterp_Lem(es[0], es[0], env, ctx, ctx');
-
-      // Evaluate the remaining expressions
-      if res0.Success? && res0.value.ret == V.Unit {
-        var Return(_, ctx0) := res0.value;
-        var Return(_, ctx0') := res0'.value;
-
-        InterpBlock_Exprs_Refl(es[1..], env, ctx0, ctx0');
-      }
-      else {
-        // Trivial
-      }
-    }
   }
 }
 
@@ -292,16 +141,16 @@ module FilterEmptyBlocks {
 
   import opened FilterCommon
 
-  type {:verify false} Expr = Syntax.Expr
+  type Expr = Syntax.Expr
 
-  function method {:verify false} FilterEmptyBlocks_Seq(es: seq<Expr>): (es': seq<Expr>)
+  function method FilterEmptyBlocks_Seq(es: seq<Expr>): (es': seq<Expr>)
     ensures Seq_All(SupportsInterp, es) ==> Seq_All(SupportsInterp, es')
     ensures |es| >= |es'|
   {
     Seq.Filter(es, IsNonEmptyBlock)
   }
 
-  function method {:verify false} FilterEmptyBlocks_Single(e: Expr): Expr
+  function method FilterEmptyBlocks_Single(e: Expr): Expr
   {
     if e.Block? then
       Expr.Block(FilterEmptyBlocks_Seq(e.stmts))
@@ -309,7 +158,7 @@ module FilterEmptyBlocks {
       e
   }
 
-  lemma {:verify false} FilterEmptyBlocks_Seq_Rel(es: seq<Expr>, env: Environment, ctx: State, ctx': State)
+  lemma FilterEmptyBlocks_Seq_Rel(es: seq<Expr>, env: Environment, ctx: State, ctx': State)
     requires Seq_All(SupportsInterp, es)
     requires EqState(ctx, ctx')
     ensures EqInterpResultValue(InterpBlock_Exprs(es, env, ctx), InterpBlock_Exprs(FilterEmptyBlocks_Seq(es), env, ctx'))
@@ -344,8 +193,8 @@ module FilterEmptyBlocks {
       }
       else {
         assert es' == es;
-        EqInterp_Refl_Lem(es[0]);
-        EqInterp_Lem(es[0], es[0], env, ctx, ctx');
+        EqInterp_Refl(es[0]);
+        EqInterp_Inst(es[0], es[0], env, ctx, ctx');
       }
     }
     else {
@@ -360,6 +209,9 @@ module FilterEmptyBlocks {
           reveal InterpBlock();
           // Doesn't work without this assertion
           assert res0 == InterpBlock(es[0].stmts, env, ctx);
+          assert es[0].stmts == [];
+          // Doesn't work without this assertion
+          assert InterpBlock(es[0].stmts, env, ctx) == InterpBlock_Exprs([], env, ctx);
         }
 
         assert es' == FilterEmptyBlocks_Seq(es[1..]);
@@ -368,8 +220,8 @@ module FilterEmptyBlocks {
       else {
         // The first expression is not filtered
 
-        EqInterp_Refl_Lem(es[0]);
-        EqInterp_Lem(es[0], es'[0], env, ctx, ctx');
+        EqInterp_Refl(es[0]);
+        EqInterp_Inst(es[0], es'[0], env, ctx, ctx');
 
         var tl := es[1..];
         var tl' := FilterEmptyBlocks_Seq(tl);
@@ -384,7 +236,7 @@ module FilterEmptyBlocks {
     }
   }
 
-  lemma {:verify false} FilterEmptyBlocks_Single_Rel(e: Expr)
+  lemma FilterEmptyBlocks_Single_Rel(e: Expr)
     ensures Tr_Expr_Rel(e, FilterEmptyBlocks_Single(e))
   {
     if e.Block? && SupportsInterp(e) {
@@ -405,7 +257,7 @@ module FilterEmptyBlocks {
       assert EqInterp(e, e');
     }
     else {
-      EqInterp_Refl_Lem(e); 
+      EqInterp_Refl(e); 
     }
   }
 }
@@ -428,9 +280,9 @@ module InlineLastBlock {
 
   import opened FilterCommon
 
-  type {:verify false} Expr = Syntax.Expr
+  type Expr = Syntax.Expr
 
-  function method {:verify false} InlineLastBlock_Seq(es: seq<Expr>): (es': seq<Expr>)
+  function method InlineLastBlock_Seq(es: seq<Expr>): (es': seq<Expr>)
     ensures Seq_All(SupportsInterp, es) ==> Seq_All(SupportsInterp, es')
     // If the last expression of a sequence of expressions is a block, inline its content.
     //
@@ -455,13 +307,13 @@ module InlineLastBlock {
       [es[0]] + InlineLastBlock_Seq(es[1..])
   }
 
-  function method {:verify false} InlineLastBlock_Single(e: Expr): Expr
+  function method InlineLastBlock_Single(e: Expr): Expr
   {
     if e.Block? then Expr.Block(InlineLastBlock_Seq(e.stmts))
     else e
   }
 
-  lemma {:verify false} InlineLastBlock_Seq_Rel(es: seq<Expr>, env: Environment, ctx: State, ctx': State)
+  lemma InlineLastBlock_Seq_Rel(es: seq<Expr>, env: Environment, ctx: State, ctx': State)
     requires forall e | e in es :: SupportsInterp(e)
     requires EqState(ctx, ctx')
     ensures forall e | e in InlineLastBlock_Seq(es) :: SupportsInterp(e)
@@ -497,8 +349,8 @@ module InlineLastBlock {
     }
     else {
       // The first expression appears in both sequences
-      EqInterp_Refl_Lem(es[0]);
-      EqInterp_Lem(es[0], es'[0], env, ctx, ctx');
+      EqInterp_Refl(es[0]);
+      EqInterp_Inst(es[0], es'[0], env, ctx, ctx');
 
       // Prove that the sequence concatenations are evaluated in a similar manner
       var tl := es[1..];
@@ -514,7 +366,7 @@ module InlineLastBlock {
   }
 
   // Rk.: modulo the names, this is exactly the same proof as for ``FilterEmptyBlocks_Single_Rel``
-  lemma {:verify true} InlineLastBlock_Single_Rel(e: Expr)
+  lemma InlineLastBlock_Single_Rel(e: Expr)
     ensures Tr_Expr_Rel(e, InlineLastBlock_Single(e))
   {
     if e.Block? && SupportsInterp(e) {
@@ -535,7 +387,7 @@ module InlineLastBlock {
       assert EqInterp(e, e');
     }
     else {
-      EqInterp_Refl_Lem(e); 
+      EqInterp_Refl(e); 
     }
   }
 }
